

Problem 1.4

$$\begin{aligned} 6x - 5y &= 10 \\ -13x + 10y &= -20 \end{aligned}$$

$$\begin{aligned} \frac{1}{-5}(0x - 5y) &= (10) \frac{1}{-5} \\ 0x - \frac{5y}{-5} &= \frac{10}{-5} \rightarrow 0x + y = -2 \end{aligned}$$

$$\left[ \begin{array}{cc|c} 6 & -5 & 10 \\ -13 & 10 & -20 \end{array} \right] \xrightarrow{2} \sim \left[ \begin{array}{cc|c} 6 & -5 & 10 \\ -1 & 0 & 0 \end{array} \right] \xrightarrow{\cdot(-1)} \sim \left[ \begin{array}{cc|c} 6 & -5 & 10 \\ 1 & 0 & 0 \end{array} \right] \xrightarrow{-6} \sim \left[ \begin{array}{cc|c} 0 & -5 & 10 \\ 1 & 0 & 0 \end{array} \right] \xrightarrow{\frac{1}{-5}} \sim \left[ \begin{array}{cc|c} 0 & 1 & -2 \\ 1 & 0 & 0 \end{array} \right]$$

Problem 3.4

$$\left[ \begin{array}{ccc|c} 2 & 6 & 15 & -12 \\ 4 & 7 & 13 & -10 \\ 3 & 6 & 12 & -9 \end{array} \right]$$

Endgültig  
Lösung  $\begin{cases} x=0 \\ y=-2 \end{cases}$

$$\left[ \begin{array}{ccc|c} 2 & 6 & 15 & -12 \\ 4 & 7 & 13 & -10 \\ 3 & 6 & 12 & -9 \end{array} \right] \xrightarrow{\frac{1}{3}} \sim \left[ \begin{array}{ccc|c} 2 & 6 & 15 & -12 \\ 4 & 7 & 13 & -10 \\ 1 & 2 & 4 & -3 \end{array} \right] \xrightarrow{-4} \sim \left[ \begin{array}{ccc|c} 0 & 2 & 7 & -6 \\ 0 & -1 & -3 & 2 \\ 1 & 2 & 4 & -3 \end{array} \right] \xrightarrow{2} \sim \left[ \begin{array}{ccc|c} 0 & 0 & 1 & -2 \\ 0 & -1 & -3 & 2 \\ 1 & 0 & -2 & 1 \end{array} \right] \xrightarrow{2} \sim \left[ \begin{array}{ccc|c} 0 & 0 & 1 & -2 \\ 0 & -1 & 0 & -4 \\ 1 & 0 & 0 & -3 \end{array} \right] \xrightarrow{\cdot(-1)} \left[ \begin{array}{ccc|c} 0 & 0 & 1 & -2 \\ 0 & 1 & 0 & 4 \\ 1 & 0 & 0 & -3 \end{array} \right]$$

Problem 3.5

$$\left[ \begin{array}{ccc|c} 2 & 3 & 5 & 21 \\ 1 & -1 & -5 & -2 \\ 2 & 1 & -1 & 11 \end{array} \right]$$

Endgültig  
Lösung  $\begin{cases} x=-3 \\ y=4 \\ z=-2 \end{cases}$

$$\left[ \begin{array}{ccc|c} 2 & 3 & 5 & 21 \\ 1 & -1 & -5 & -2 \\ 2 & 1 & -1 & 11 \end{array} \right] \xrightarrow{-2} \sim \left[ \begin{array}{ccc|c} 0 & 5 & 15 & 25 \\ 1 & -1 & -5 & -2 \\ 0 & 3 & 9 & 15 \end{array} \right] \xrightarrow{\frac{1}{3}} \sim \left[ \begin{array}{ccc|c} 0 & 1 & 3 & 5 \\ 1 & -1 & -5 & -2 \\ 0 & 1 & 3 & 5 \end{array} \right] \xrightarrow{-1} \sim \left[ \begin{array}{ccc|c} 0 & 0 & 0 & 0 \\ 1 & -1 & -5 & -2 \\ 0 & 1 & 3 & 5 \end{array} \right] \xrightarrow{1} \sim \left[ \begin{array}{ccc|c} 0 & 0 & 0 & 0 \\ 1 & 0 & -2 & 3 \\ 0 & 1 & 3 & 5 \end{array} \right]$$

$$\begin{aligned} x &= 9 \\ y &= -4 \\ z &= 3 \end{aligned}$$

$$\begin{aligned} 2x + 3y + 5z &= 21 \\ x - y - 5z &= -2 \\ 2x + y - z &= 11 \end{aligned}$$

$$\begin{aligned} 0 &= 0 \\ x - y - 5z &= -2 \\ y + 3z &= 5 \end{aligned}$$

$$\begin{aligned} 0 &= 0 \\ x - 2z &= 3 \\ y + 3z &= 5 \end{aligned} \rightarrow \begin{aligned} x &= 3 + 2z \\ y &= 5 - 3z \end{aligned}$$

$$\begin{aligned} x &= 3 + 2t \\ y &= 5 - 3t \\ z &= t, t \in \mathbb{R} \end{aligned}$$

Endlich viele  
Lösungen

$$\begin{aligned} z &= 3 \\ x &= 9 \\ y &= -4 \end{aligned}$$

Problem 3.6

$$\left[ \begin{array}{ccc|c} 4 & -2 & 2 & 5 \\ -6 & 3 & -3 & -2 \\ 10 & -5 & 9 & 4 \end{array} \right]$$

$$\left[ \begin{array}{ccc|c} 4 & -2 & 2 & 5 \\ -6 & 3 & -3 & -2 \\ 10 & -5 & 9 & 4 \end{array} \right] \xrightarrow{7} \sim \left[ \begin{array}{ccc|c} 4 & -2 & 2 & 5 \\ -6 & 3 & -3 & -2 \\ 4 & -2 & 6 & 2 \end{array} \right] \xrightarrow{-2} \sim \left[ \begin{array}{ccc|c} 4 & -2 & 2 & 5 \\ -6 & 3 & -3 & -2 \\ 0 & 0 & 4 & -3 \end{array} \right] \xrightarrow{2} \sim \left[ \begin{array}{ccc|c} 4 & -2 & 2 & 5 \\ -2 & 1 & -1 & 3 \\ 0 & 0 & 4 & -3 \end{array} \right] \xrightarrow{2} \sim \left[ \begin{array}{ccc|c} 0 & 0 & 0 & 11 \\ -2 & 1 & -1 & 3 \\ 0 & 0 & 4 & -3 \end{array} \right] \text{ STOP}$$

Contradiction  
 $0 = 11 \rightarrow$  keine Lösungen

$$\left[ \begin{array}{ccc|c} 4 & -2 & 2 & 5 \\ -6 & 3 & -3 & -2 \\ 10 & -5 & 9 & 4 \end{array} \right] \xrightarrow{\frac{1}{2}} \sim \left[ \begin{array}{ccc|c} 4 & -2 & 2 & 5 \\ 4 & -2 & 2 & -3 \\ 10 & -5 & 9 & 4 \end{array} \right] \xrightarrow{-2} \sim \left[ \begin{array}{ccc|c} 4 & -2 & 2 & 5 \\ 0 & 0 & 0 & -8 \\ 10 & -5 & 9 & 4 \end{array} \right]$$

$$\begin{aligned} 4x - 2y + 2z &= 5 \\ 4x - 2y + 2z &= -3 \\ 10x - 5y + 9z &= 4 \end{aligned}$$